SpinLock/BruteForceAutomation.thy
@@ -1,0 +1,96 @@
+theory BruteForceAutomation
+imports "../HeapLang/WeakestPrecondition"
+begin
+
+subsection \<open>Brute force automation\<close>
+context wp_rules begin
+(*
+  General idea: iterate over all hypotheses (i.e. all single iprop terms connected by separating
+  conjunctions), move them to the top and try all rules in a brute force approach.
+  Only backtrack to the next hypothesis if there is nothing that can be done for the
+  current hypothesis (plus goal).
+  
+  It might help to use a normal form of sorts (similarly to Diaframe) but we try to make this 
+  approach work without such an extra step.
+*)
+
+subsubsection \<open>Rule setup\<close>
+text \<open>All rules operate directly on the top level hypothesis.\<close>
+
+lemmas splitting_rules = split_rule can_be_split_sepL persistent_dupl' persistent_dupl_split
+
+lemmas intro_rules = upred_wandI upred_wand_holdsI
+
+lemmas single_goal_framing = upred_entails_refl upred_entails_trans[OF upred_weakeningR split_last_frame]
+  split_last_frame
+
+lemmas multi_goal_framing = upred_frame framing'' framing'
+
+lemmas single_hyp_framing = upred_wand_goal framing
+
+lemmas pure_goal_lifting = upred_pureI upred_sep_pure
+lemmas pure_hypothesis_lifting = upred_pure_impl
+
+lemmas fupd_elim_hyps = elim_modal_entails'[OF elim_modal_fupd]
+  elim_modal_entails[OF elim_modal_fupd]
+  elim_modal_entails[OF elim_modal_fupd_wp_atomic]
+  elim_modal_entails'[OF elim_modal_fupd_wp_atomic]
+
+lemmas bupd_elim = upred_entails_trans[OF upd_fupd[to_entailment]]
+  upred_entails_substE[OF upd_fupd[to_entailment]]
+  
+lemmas later_elim_hyps = upred_later_mono_extR upred_later_mono
+  elim_modal_entails'[OF elim_modal_timeless']
+  elim_modal_entails[OF elim_modal_timeless']
+  upred_entails_trans[OF upred_entail_eqR[OF upred_later_sep] upred_later_mono]
+
+lemmas existential_elim_hyps = upred_existsE_ext upred_existsE'
+
+lemmas existential_elim_goal = upred_exists_lift[OF exI] upred_exists_lift'[OF exI]
+
+lemmas universal_elim_goal = upred_forallI
+
+lemmas wp_symbolic_execution_steps = upred_entails_trans[OF _ wp_pure_step_later[OF pure_exec_beta, simplified]]
+  upred_entails_trans[OF _  wp_pure_step_later[OF pure_exec_fst, simplified]] 
+  upred_entails_trans[OF _ wp_pure_step_later[OF pure_exec_snd, simplified]] 
+  wp_load wp_let_bind' wp_alloc' wp_store' upred_entails_trans[OF _ wp_value]
+  
+lemmas additional_simps = upred_exists_eq_sep upred_exists_eq_sep' upred_pure_sep_conj' 
+  upred_exists_eq_sepR upred_exists_eq_sepR' subst'_def upred_holds_entails
+declare additional_simps[iris_simp]
+
+lemmas last_resort_drop_goal_modality = upred_persis_mono[where ?P=upred_emp, unfolded emp_rule]
+  upred_entails_trans[OF _ upred_laterI] upred_entails_trans[OF _ fupd_intro[to_entailment]]
+  upred_entails_trans[OF _ upred_entails_trans[OF upred_laterI upred_entail_eqL[OF upred_later_sep]]]
+  
+subsubsection \<open>Brute force iteration methods\<close>
+
+method framing =
+  ((rule single_hyp_framing, fast intro: frame_rule, iris_simp?)
+  | auto simp: iris_simp intro!: log_prog_rule single_goal_framing multi_goal_framing);
+  is_entailment
+
+text \<open>Try all possible rules and steps for the given hypothesis.\<close>
+method brute_force_hyp =
+  (auto simp: iris_simp 
+  intro!: pure_goal_lifting universal_elim_goal existential_elim_hyps upred_universal_wand
+    intro_rules fupd_elim_hyps bupd_elim later_elim_hyps(1,2) existential_elim_goal pure_hypothesis_lifting
+  intro: log_prog_rule later_elim_hyps(3-5)
+  | framing)
+    
+text \<open>Apply brute force search to all hypotheses by destructuring the antecedent.\<close>
+method brute_force_hyps for hyps :: iprop =
+  match (hyps) in "rest\<^emph>hyp" for rest hyp :: iprop \<Rightarrow> \<open>(move_sepL hyp, brute_force_hyp) | brute_force_hyps rest\<close>
+  \<bar> _ \<Rightarrow> \<open>(move_sepL hyps, brute_force_hyp)
+      | step intro: last_resort_drop_goal_modality wp_symbolic_execution_steps
+      | (rule framing_emp, fast intro!: log_prog_rule, is_entailment)\<close>
+
+text \<open>Get the antecedent from the conclusion entailment term and start the iteration process.\<close>
+method iterate_hyps_safe for concl_trm :: bool = 
+  match (concl_trm) in "hyps\<turnstile>_" for hyps :: iprop \<Rightarrow> \<open>brute_force_hyps hyps\<close>
+
+text \<open>Iterate over the hypotheses and apply possible rules in a brute force manner.\<close>
+method iterate_hyps =
+  iris_simp; get_concl "BruteForceAutomation.wp_rules.iterate_hyps_safe"
+end
+end
